seiostar/QTypes.fst
@@ -12,19 +12,21 @@ noeq
 type type_quotation : Type0 -> Type u#1 =
 | QUnit : #ref:(unit -> Type0) -> type_quotation (x:unit{ref x})
 | QBool : #ref:(bool -> Type0) -> type_quotation (x:bool{ref x})
-| QNat  : type_quotation nat
+| QNat  : #ref:(nat -> Type0) -> type_quotation (x:nat{ref x})
 | QFileDescriptor : #ref:(file_descr -> Type0) -> type_quotation (x:file_descr{ref x})
 | QString : #ref:(string -> Type0) -> type_quotation (x:string{ref x})
 | QArr : #t1:Type ->
          #t2:Type ->
          type_quotation t1 ->
          type_quotation t2 ->
-         type_quotation (t1 -> t2)
+         #ref:((t1 -> t2) -> Type0) ->
+         type_quotation (f:(t1 -> t2){ref f})
 | QArrIO : #t1:Type ->
          #t2:Type ->
          type_quotation t1 ->
          type_quotation t2 ->
-         type_quotation (t1 -> io t2)
+         #ref:((t1 -> io t2) -> Type0) ->
+         type_quotation (f:(t1 -> io t2){ref f})
 | QPair : #t1:Type ->
           #t2:Type ->
           type_quotation t1 ->
@@ -44,8 +46,8 @@ let test_match t (tq:type_quotation t) = (** why does this work so well? **)
   | QBool #ref -> assert (t == x:bool{ref x})
   | QFileDescriptor #ref -> assert (t == x:file_descr{ref x})
   | QString #ref -> assert (t == x:string{ref x})
-  | QArr #t1 #t2 _ _ -> assert (t == (t1 -> t2))
-  | QArrIO #t1 #t2 _ _ -> assert (t == (t1 -> io t2))
+  | QArr #t1 #t2 _ _ #ref -> assert (t == f:(t1 -> t2){ref f})
+  | QArrIO #t1 #t2 _ _ #ref -> assert (t == f:(t1 -> io t2){ref f})
   | QPair #t1 #t2 _ _ #ref -> assert (t == (x:(t1 & t2){ref x}))
   | QSum #t1 #t2 _ _ #ref -> assert (t == (x:(either t1 t2){ref x}))
   | QUnit -> assert (t == unit)
@@ -56,7 +58,7 @@ let test_match t (tq:type_quotation t) = (** why does this work so well? **)
   | QArrIO #t1 #t2 _ _ -> assert (t == (t1 -> io t2))
   | QPair #t1 #t2 _ _ -> assert (t == (t1 & t2))
   | QSum #t1 #t2 _ _ -> assert (t == either t1 t2)
-  | QNat -> assert (t == nat)
+  | QNat #ref -> assert (t == x:nat{ref x})
 
 let rec type_quotation_to_typ #s (qt:type_quotation s) : typ =
   match qt with
@@ -115,18 +117,15 @@ let thetaP_io_map_id (#a:Type) (f:a -> a) (m:io a) (h:history) (lt:local_trace h
       (ensures (thetaP (io_map f m) h lt r <==> thetaP m h lt r)) =
   theta_io_map_id f m
 
-// let subQtype_of (a b:qType) : Type0 =
-//   get_Type a `subtype_of` get_Type b
-
 let qUnitR ref : qType = (| _, QUnit #ref |)
 let qBoolR ref : qType = (| _, QBool #ref |)
 let qFileDescrR ref : qType = (| _, QFileDescriptor #ref |)
 let qStringR ref : qType = (| _, QString #ref |)
 let qSumR t1 t2 ref : qType = (| _, QSum (get_rel t1) (get_rel t2) #ref |)
 let qPairR t1 t2 ref : qType = (| _, QPair (get_rel t1) (get_rel t2) #ref |)
-
-//let qArrR (t1 t2:qType) post : qType = (| _, QArr (get_rel t1) (get_rel t2) #post |)
-//let qArrIOR (t1 t2:qType) post : qType = (| _, QArrIO (get_rel t1) (get_rel t2) #post |)
+let qArrR t1 t2 ref : qType = (| _, QArr (get_rel t1) (get_rel t2) #ref |)
+let qArrIOR t1 t2 ref : qType = (| _, QArrIO (get_rel t1) (get_rel t2) #ref |)
+let qNatR ref : qType = (| _, QNat #ref |)
 
 let qUnit : qType = qUnitR (fun _ -> True)
 let qBool : qType = qBoolR (fun _ -> True)
@@ -135,16 +134,12 @@ let qString : qType = qStringR (fun _ -> True)
 
 // let qRef (t:qType) (ref: get_Type t -> Type0) : qType =
 //   (| _, QRefinement (get_rel t) ref |)
-let (^->) (t1 t2:qType) : qType =
-  (| _, QArr (get_rel t1) (get_rel t2) |)
-let (^->!@) (t1 t2:qType) : qType =
-  (| _, QArrIO (get_rel t1) (get_rel t2) |)
-let (^*) (t1 t2:qType) : qType =
-  (| _, QPair (get_rel t1) (get_rel t2) #(fun _ -> True) |)
-let (^+) (t1 t2:qType) : qType =
-  (| _, QSum (get_rel t1) (get_rel t2) #(fun _ -> True) |)
+let (^->) (t1 t2:qType) : qType = (| _, QArr (get_rel t1) (get_rel t2) #(fun _ -> True) |)
+let (^->!@) (t1 t2:qType) : qType = (| _, QArrIO (get_rel t1) (get_rel t2) #(fun _ -> True) |)
+let (^*) (t1 t2:qType) : qType = (| _, QPair (get_rel t1) (get_rel t2) #(fun _ -> True) |)
+let (^+) (t1 t2:qType) : qType = (| _, QSum (get_rel t1) (get_rel t2) #(fun _ -> True) |)
 
-let qNat : qType = (| _, QNat |)
+let qNat : qType = qNatR (fun _ -> True)
 
 let qResexn (t1:qType) : qType = t1 ^+ qUnit
 
@@ -173,9 +168,9 @@ let ref_of (a:qType) : ref_type a -> Type0 =
   | QString #ref -> ref
   | QPair _ _ #ref -> ref
   | QSum _ _ #ref -> ref
-  | QNat -> (fun _ -> True)
-  | QArr _ _ -> (fun _ -> True)
-  | QArrIO _ _ -> (fun _ -> True)
+  | QNat #ref -> ref
+  | QArr _ _ #ref -> ref
+  | QArrIO _ _ #ref -> ref
 
 let change_refinement (t:qType) (ref: ref_type t -> Type0) : qType =
   match get_rel t with
@@ -185,9 +180,9 @@ let change_refinement (t:qType) (ref: ref_type t -> Type0) : qType =
   | QString -> qStringR ref
   | QSum qt1 qt2 -> qSumR (pack qt1) (pack qt2) ref
   | QPair qt1 qt2 -> qPairR (pack qt1) (pack qt2) ref
-  | QNat -> t
-  | QArr _ _ -> t
-  | QArrIO _ _ -> t
+  | QNat -> qNatR ref
+  | QArr qt1 qt2 -> qArrR (pack qt1) (pack qt2) ref
+  | QArrIO qt1 qt2 -> qArrIOR (pack qt1) (pack qt2) ref
 
 let q_io_args (o:io_ops) : qType =
   match o with
